tests/LibC/JS.TypedObjects.fsti
@@ -11,12 +11,15 @@ module U = JS.Primitives.Unsafe
 module L = FStar.List.Tot
 module T = FStar.Tactics
 
+irreducible let normMark = ()
+
 (** A key can be either a string or a integer. TODO: support JS numbers and symbols. *)
 type js_key
   = | StringJsKind: string -> js_key
     | IntJsKind:         int -> js_key
 
 (** Converts a `js_key` to a js_any *)
+[@@normMark]
 let js_any_of_js_key (k: js_key): Js U.js_any
   = match k with
   | StringJsKind s -> U.inject (U.to_js_string s)
@@ -24,66 +27,87 @@ let js_any_of_js_key (k: js_key): Js U.js_any
 
 (***** Types for typed objects. *)
 (** TODO documentation. *)
+[@@normMark]
 noeq type js_obj_d = {
-  props: js_key -> Type;
-  callable: list (list Type * Type)
+  [@@@normMark] props: js_key -> Type;
+  [@@@normMark] fn_overloadings: list (list Type * Type)
 }
 (** A typed object is of type `js_obj f`, with `f` a map from keys of type `js_key` to types.
     Keys that does not belong to an object are to be mapped to `undefinedType`. *)
-val js_obj: js_obj_d -> Type
+[@@normMark]
+val js_obj': js_obj_d u#a u#b u#c -> Type u#c
 (** The type of the `undefined` JavaScript value. *)
 val undefinedType: Type
 (** The type of the `null` JavaScript value. *)
 val nullType: Type
 
+unfold let js_obj d = norm [primops; iota; delta_attr [`%normMark]; delta_only [`%L.map;`%op_Equality]; zeta] (js_obj' d)
+
 (** Utility function. *)
-let rec list_to_map (#k:eqtype) (l: list (k * Type)): k -> Type
+[@@normMark]
+let rec list_to_map_rec (#key:eqtype) (l: list (key * Type)) (k: key): Type
   = match l with
-  | [] -> (fun _ -> undefinedType)
-  | (k,t)::tl  -> (fun k' -> if k=k' then t
-                                else list_to_map tl k')
+  | [] -> undefinedType
+  | (k',t)::tl -> if k=k' then t
+                else list_to_map_rec tl k
+[@@normMark]
+let list_to_map (#key:eqtype) (l: list (key * Type)) (k: key): Type
+  = match l with
+  | [] -> undefinedType
+  | (k0,v0)::[] -> if k0=k then v0 else undefinedType
+  | (k0,v0)::(k1,v1)::[] -> if k0=k then v0 else if k1=k then v1 else undefinedType
+  | (k0,v0)::(k1,v1)::(k2,v2)::[] -> if k0=k then v0 else if k1=k then v1 else if k2=k then v2 else undefinedType
+  | _ -> list_to_map_rec l k
 
 (***** Operations on typed objects. *)
 (** Gets the property `k` (of type `js_key`) of an object `o`. Prefer (.[]) bellow. *)
-val get (#d: _) (o: js_obj d) (k: js_key): Js (d.props k)
+val get (#d: _) (o: js_obj' d) (k: js_key): Js (d.props k)
 (** Sets the property `k` (of type `js_key`) of an object `o` to the value `v`. Prefer (.[]<-) bellow. *)
-val set (#d: _) (o: js_obj d) (k: js_key) (v: d.props k): Js unit
-(** TODO doc. *)
-unfold let desc_obj (map: list (string * (t: Type & t))) callable =
-  normalize_term ({
-    props = list_to_map (L.map (fun (k, (|t, _|)) -> (StringJsKind k,t)) map);
-    callable = callable
-  })
+val set (#d: _) (o: js_obj' d) (k: js_key) (v: d.props k): Js unit
+(** Utility function converting property specifications and overaloadings to `obj_d`. *)
+[@@normMark]
+unfold let obj_d_of (map: list (string * Type)) fn_overloadings =
+  {
+    props = list_to_map (L.map (fun (k, t) -> (StringJsKind k,t)) map);
+    fn_overloadings = fn_overloadings
+  }
 (** Creates a typed object litteral. *)
 val obj (map: list (string * (t: Type & t)))
-  : Js (js_obj (desc_obj map []))
+  : Js (js_obj (obj_d_of (L.map (fun (k, (|t, _|)) -> (k,t)) map) []))
 
 (***** Overloaded operations on typed objects. *)
 (** Typeclass for types that can be coerced into a `js_key`. *)
-class has_key_coercion (k: Type) = { key_coercion: k -> js_key }
+[@@normMark]
+class has_key_coercion (k: Type) = { [@@@normMark] key_coercion: k -> js_key }
 
 (** Values of type `string` can be coerced as `js_key`s. *)
+[@@normMark]
 instance string_key_coercion: has_key_coercion string = { key_coercion = (fun s -> StringJsKind s) }
 (** Values of type `int` can be coerced as `js_key`s. *)
+[@@normMark]
 instance int_key_coercion: has_key_coercion int = { key_coercion = (fun i -> IntJsKind i) }
 
+
 (** The expression `o.[k] <- v` sets the property `k` of object `o` to value `v`. *)
-let (.[]<-) #d #key {| has_key_coercion key |} (o: js_obj d) (k: key): normalize_term (d.props (key_coercion k)) -> Js unit
+let (.[]<-) #d #key {| has_key_coercion key |} ($o: js_obj' d) (k: key)
+  : norm [primops; iota; delta_attr [`%normMark]; delta_only [`%L.map;`%op_Equality]; zeta] (d.props (key_coercion k))
+  -> Js unit
   = fun v -> set o (key_coercion k) v
 
 (** The expression `o.[k]` gets the property `k` of object `o`. *)
-let (.[]) #d #key {| has_key_coercion key |} (o: js_obj d) (k: key): Js (normalize_term (d.props (key_coercion k)))
+let (.[]) #d #key {| has_key_coercion key |} ($o: js_obj' d) ($k: key)
+  : Js (norm [primops; iota; delta_attr [`%normMark]; delta_only [`%L.map;`%op_Equality]; zeta] (d.props (key_coercion k)))
   = get o (key_coercion k)
 
 val call
   (#d: _) (nth: nat) (o: js_obj d) (this: U.js_any)
   (args: list (t: Type & t) {
-    match L.nth d.callable nth with
+    match L.nth d.fn_overloadings nth with
     | Some (inT, outT) -> 
           L.length args == L.length inT
         /\ (forall i. dfst (L.index args i) `subtype_of` L.index inT i)
     | None -> False
-  }): Js (snd (Some?.v (L.nth d.callable nth)))
+  }): Js (snd (Some?.v (L.nth d.fn_overloadings nth)))
 
 (***** From n-tuples to lists, TODO move somewhere else. *)
 class tup_to_list (a: Type) = {
@@ -92,6 +116,11 @@ class tup_to_list (a: Type) = {
       L.length extract_type_list == L.length l
     /\ (forall i. dfst (L.index l i) == L.index extract_type_list i)
   })
+}
+
+instance tup1_to_list a: tup_to_list a = {
+  extract_type_list = [a];
+  extract_values = (fun x -> [(|a,x|)]);
 }
 
 instance tup2_to_list a b: tup_to_list (a * b) = {
@@ -125,114 +154,21 @@ instance tup7_to_list a b c d e f g: tup_to_list (a*b*c*d*e*f*g) = {
                       ]);
 }
 
-(***** Util. functions, TODO move somewhere else. *)
-
-let subtype_tac (t0 t1: Type): T.Tac bool =
-  let binder = T.fresh_binder (quote t0) in
-  let body = T.Tv_AscribedT (T.binder_to_term binder) (quote t1) None in
-  let t = T.pack (T.Tv_Abs binder (T.pack body)) in
-  Some? (T.trytac (fun _ -> T.tc (T.top_env ()) t))
-
-let rec tfilter_h (ref: list 'a) (f: (x:'a{L.memP x ref}) -> T.Tac bool) (l: list 'a{forall i. L.memP i l ==> L.memP i ref})
-  : T.Tac (l': list 'a {forall x. L.memP x l' ==> L.memP x ref}) 
-  = match l with
-  | [] -> []
-  | hd::tl -> if f hd then hd::(tfilter_h ref f tl) else tfilter_h ref f tl
-
-let tfilter (ref: list 'a) (f: (x:'a{L.memP x ref}) -> T.Tac bool)
-  : T.Tac (l': list 'a {forall x. L.memP x l' ==> L.memP x ref}) 
-  = tfilter_h ref f ref
-
-let rec withIndex_h
-  (ref:list 'a)
-  (n:nat{n<=L.length ref})
-  (l:list 'a {n + L.length l = L.length ref})
-  : Tot (r:list (nat*'a) {(forall x. L.memP x r ==> fst x < L.length ref) /\ L.length r == L.length l}) (decreases l)
-= match l with
-| [] -> []
-| hd::tl -> (n, hd)::withIndex_h ref (n+1) tl
-
-let withIndex (l: list 'a): r:list (nat * 'a){
-    L.length l == L.length r /\ (forall x. L.memP x r ==> fst x < L.length l)
-  } = withIndex_h l 0 l
-
-
-let rec filter_lemma (l: list 'a) f
-  : Lemma (forall x. L.memP x (L.filter f l) ==> L.memP x l)
-          [SMTPat (L.filter f l)]
-  = match l with | [] -> () | _::tl -> filter_lemma tl f
-let rec lemma_nth (l: list 'a) (n: nat)
-  : Lemma (requires n < L.length l) 
-          (ensures 
-              (Some? (L.nth l n))
-            /\ (Some?.v (L.nth l n) == L.index l n)
-          )
-          [SMTPat (L.nth l n)]
-  = match l,n with
-  | _, 0 | [], _ -> ()
-  | hd::tl, _ -> lemma_nth tl (n-1)
-
+open Js.TypedObjects.Utils
 (***** Calling overloaded JavaScript funtions. *)
-(** Meta-program that choose the appropriate overloading for a JavaScript function. 
-    Given `sigs` a list of overloadings, and `inputs` the inputs arguments, returns the index of most appropriate overloading (in `sigs`). *)
-let resolve_fun_signature
-  (sigs: list (list Type * Type)) (inputs: list Type)
-  : T.Tac (n:int{n < L.length sigs})
-  = let len = L.length inputs in
-    let sigs': l: list (nat * (list Type * Type)) {
-        forall x. L.memP x l ==> fst x < L.length sigs
-      } = withIndex sigs in
-    assert (L.length sigs' == L.length sigs);
-    let correct_size: l: list (nat * (list Type * Type)) {
-        forall x. L.memP x l ==> (
-            L.length (fst (snd x)) == len
-          /\ fst x < L.length sigs'
-        )
-      }
-      = L.filter (fun (i, (inT, outT)) -> L.length inT = len) sigs' in
-    if Nil? correct_size then 
-      T.fail "Bad arity for JS function.";
-    if len = 0 && L.length correct_size <> 1 then
-      T.fail "JS function call: cannot decide between TODO";
-    let rec while_multiple (nb len: nat) 
-      (inputs:_{L.length inputs == len}) (i: nat{i<=len})
-      (l: list (nat * (list Type * Type)) {
-        forall i. L.memP i l ==> (
-          L.length (fst (snd i)) == len /\
-          fst i < nb
-        )
-      })
-     : T.Tac (n: nat{n < nb})
-     = if i=len then T.fail "JS function call: could not distinguish."
-       else match l with
-       | [] -> T.fail "JS function call: wrong type."
-       | hd::[] -> fst hd
-       | _ -> let f (tt: _ {L.memP tt l}): T.Tac bool = subtype_tac (L.index inputs i) (L.index (fst (snd tt)) i) in
-             while_multiple nb len inputs (i+1) (tfilter l f)
-    in
-    while_multiple (L.length sigs') len inputs 0 correct_size
-
-(** Meta-programs that crafts a term w.r.t. `resolve_fun_signature`. *)
-let compute_fun_signature
-  (sigs: list (list Type * Type)) (inputs: list Type)
-  : T.Tac unit
-  = let n = resolve_fun_signature sigs inputs in
-    let n = quote n in
-    T.exact n
-
 (** Calling a overloaded function `o` with arguments `v`.
     The meta-argument `nth` can be set manualy: the `nth` overloading of `o` will be called. *)
 let call_overloaded
   (#d: _)
   (#inTup: Type) {| i: tup_to_list inTup |}
-  (#[compute_fun_signature d.callable i.extract_type_list]nth: nat {nth < L.length d.callable})
+  (#[compute_fun_signature d.fn_overloadings i.extract_type_list]nth: nat {nth < L.length d.fn_overloadings})
   (o: js_obj d) (this: U.js_any)
   (v: inTup {normalize_term(
-    let inputs, output = L.index d.callable nth in
+    let inputs, output = L.index d.fn_overloadings nth in
     L.length i.extract_type_list == L.length inputs /\
     (forall j. L.index i.extract_type_list j `subtype_of` L.index inputs j)
   )})
-  : Js (normalize_term (snd (L.index d.callable nth)))
+  : Js (normalize_term (snd (L.index d.fn_overloadings nth)))
   = let args = i.extract_values v in
     call #d nth o this args
 
@@ -240,23 +176,13 @@ let call_overloaded
 let (.())
   (#d: _)
   (#inTup: Type) {| i: tup_to_list inTup |}
-  (#[compute_fun_signature d.callable i.extract_type_list]nth: nat {nth < L.length d.callable})
+  (#[compute_fun_signature d.fn_overloadings i.extract_type_list]nth: nat {nth < L.length d.fn_overloadings})
   (o: js_obj d)
   (v: inTup {normalize_term (
-    let inputs, output = L.index d.callable nth in
+    let inputs, output = L.index d.fn_overloadings nth in
     L.length i.extract_type_list == L.length inputs /\
     (forall j. L.index i.extract_type_list j `subtype_of` L.index inputs j)
   )}) = call_overloaded #d #inTup #i #nth o U.undefined v
 
-let test () =
-  let l = [
-              ("a", (|int, 3|));
-              ("b", (|int, 34|));
-          ] in
-  let o: js_obj (desc_obj l []) = obj l in
-  let o: js_obj (desc_obj l [
-    ([int;int], string)
-  ]) = magic () in
-  o.["a"] <- (o.["a"] + o.["b"]);
-  let x: string = o.(4,5) in
-  ()
+val coerce (#d: js_obj_d) (o: U.js_any): js_obj d
+
