tests/LibC/JS.TypedObjects.Tests.fst
@@ -1,0 +1,39 @@
+module JS.TypedObjects.Tests
+
+open JS.Effect
+open JS.TypedObjects
+
+// TODO: Without `Js _` effect annoation this fails with
+//       "Expected 'τ' but … was of type 'τ <: Type'"
+[@@expect_failure [12]]
+let test0 () =
+  let o0: js_obj (obj_d_of ["a", int; "b", int] []) = obj ["a", (|int, 3|); "b", (|int, 34|)] in
+  let o: js_obj (obj_d_of ["o",js_obj (obj_d_of ["a", int; "b", int] [])] []) = obj ["o",(|js_obj (obj_d_of ["a", int; "b", int] []), o0|)] in
+  let xx: js_obj (obj_d_of ["a", int; "b", int] []) = o.["o"] in
+  ()
+
+let test1 (): Js _ =
+  let o0 = obj ["a", (|int, 3|); "b", (|int, 34|)] in
+  let o = obj ["o",(|js_obj (obj_d_of ["a", int; "b", int] []), o0|)] in
+  let y = o.["o"] in
+  let xx = o.["o"] in
+  ()
+
+assume val test_o: js_obj (obj_d_of ["a",int;"b",int] [
+    ([int;int;int], string);
+    ([int;int], string);
+    ([int;string], string);
+    ([nat], string);
+    ([int], string);
+    ([string], string)
+  ])
+
+let test2 (): Js _ =
+  let a = obj ["a", (|int, 3|); "b", (|int, 34|)] in
+  let b = obj ["c", (|js_obj (obj_d_of ["a",int;"b",int] []), a|)] in
+  let x: js_obj (obj_d_of ["a",int;"b",int] []) = b.["c"] in
+  let x = x.["b"] in
+  test_o.["a"] <- (test_o.["a"] + test_o.["b"]);
+  let x: string = test_o.(4,"x") in
+  ()
+
