tests/LibC/Js.TypedObjects.Utils.fst
@@ -1,0 +1,187 @@
+module Js.TypedObjects.Utils
+
+module U = JS.Primitives.Unsafe
+module L = FStar.List.Tot
+module T = FStar.Tactics
+module S = FStar.String
+
+let debug_subtype_tac = false
+(** Decide wether a type is a subtype of another.
+    The result can be wrong; i.e. int is seen as a subtype of nat :(
+    But this is enough for choosing a correct overloading.
+  *)
+let subtype_tac (t0 t1: Type): T.Tac bool =
+  let t0_ = T.norm_term [primops; iota; delta; zeta] (quote t0) in
+  let t1_ = T.norm_term [primops; iota; delta; zeta] (quote t1) in
+  let expr = T.pack (T.mk_app (`magic) [t0_,T.Q_Implicit;(`()),T.Q_Explicit]) in
+  let ascribtion = T.Tv_AscribedT expr t1_ None in
+  let t = T.pack ascribtion in
+  let r = T.trytac (fun _ -> T.tc (T.top_env ()) t) in
+  if debug_subtype_tac && Some? r then 
+    T.print ( "[subtype_tac] tc result: " ^ T.term_to_string (Some?.v r));
+  let r = Some? r in
+  if debug_subtype_tac then (
+    T.print ( "[subtype_tac] crafted term is: "
+            ^  "`" ^ T.term_to_string (quote t) ^  "`"
+            );
+    T.print ( "[subtype_tac] `subtype_tac ("
+            ^ T.term_to_string t0_^") ("
+            ^ T.term_to_string t1_^")` ↝ "
+            ^ string_of_bool r
+            )
+  );
+  r
+
+#push-options "--print_implicits"
+let _ = 
+  // assert (true) by (
+  T.run_tactic (fun _ ->
+    T.guard (subtype_tac int int);
+    T.guard (subtype_tac nat int);
+    T.guard (subtype_tac (x:int{x > 323}) int);
+    T.guard (not (subtype_tac string nat));
+    // :(
+    T.guard (subtype_tac int nat);
+    ()
+  )
+#pop-options
+
+// [F*] TAC>> [subtype_tac] `subtype_tac (Prims.int <: Prims.Tot Type0) (Prims.int <: Prims.Tot Type0)` ↝ true
+// [F*] TAC>> [subtype_tac] `subtype_tac (Prims.int <: Prims.Tot Type0) (Prims.string <: Prims.Tot Type0)` ↝ true
+
+
+let rec tfilter_h (ref: list 'a) (f: (x:'a{L.memP x ref}) -> T.Tac bool) (l: list 'a{forall i. L.memP i l ==> L.memP i ref})
+  : T.Tac (l': list 'a {forall x. L.memP x l' ==> L.memP x ref}) 
+  = match l with
+  | [] -> []
+  | hd::tl -> if f hd then hd::(tfilter_h ref f tl) else tfilter_h ref f tl
+
+let tfilter (ref: list 'a) (f: (x:'a{L.memP x ref}) -> T.Tac bool)
+  : T.Tac (l': list 'a {forall x. L.memP x l' ==> L.memP x ref}) 
+  = tfilter_h ref f ref
+
+let rec withIndex_h
+  (ref:list 'a)
+  (n:nat{n<=L.length ref})
+  (l:list 'a {n + L.length l = L.length ref})
+  : Tot (r:list (nat*'a) {(forall x. L.memP x r ==> fst x < L.length ref) /\ L.length r == L.length l}) (decreases l)
+= match l with
+| [] -> []
+| hd::tl -> (n, hd)::withIndex_h ref (n+1) tl
+
+let withIndex (l: list 'a): r:list (nat * 'a){
+    L.length l == L.length r /\ (forall x. L.memP x r ==> fst x < L.length l)
+  } = withIndex_h l 0 l
+
+
+let rec filter_lemma (l: list 'a) f
+  : Lemma (forall x. L.memP x (L.filter f l) ==> L.memP x l)
+          [SMTPat (L.filter f l)]
+  = match l with | [] -> () | _::tl -> filter_lemma tl f
+let rec lemma_nth (l: list 'a) (n: nat)
+  : Lemma (requires n < L.length l) 
+          (ensures 
+              (Some? (L.nth l n))
+            /\ (Some?.v (L.nth l n) == L.index l n)
+          )
+          [SMTPat (L.nth l n)]
+  = match l,n with
+  | _, 0 | [], _ -> ()
+  | hd::tl, _ -> lemma_nth tl (n-1)
+
+
+
+(** Meta-program that chooses the appropriate overloading for a JavaScript function. 
+    Given `sigs` a list of overloadings, and `inputs` the inputs arguments, returns the index of most appropriate overloading (in `sigs`). *)
+#push-options "--z3rlimit 400"
+let rec while_multiple (error_header: nat -> string) (inputs_str: _ -> T.Tac _) (nb: nat) (len: nat)
+      (inputs:_{L.length inputs == len}) (i: nat{i<=len})
+      (l: list (nat * (list Type * Type)) {
+        ( forall i. L.memP i l ==> (
+            L.length (fst (snd i)) == len /\
+            fst i < nb
+          ))
+        /\ Cons? l
+      })
+     : T.Tac (n: nat{n < nb})
+     = if i=len then
+          match l with
+        | [hd] -> fst hd 
+        | _::_ ->
+          T.fail ( error_header 3 ^ "A JavaScript function was called with "^string_of_int len^" arguments"
+                 ^ ", but it has multiple overloadings with exactly "^string_of_int len^" arguments. "
+                 ^ "The meta-program was not able to distinguish between them: you should "
+                 ^ "set manually the meta-argument `nth` when calling the function."
+                 ^ "The "^string_of_int len^"-arguments overloadings of this JavaScript function are:\n"
+                 ^ S.concat "\n" (T.map (fun (nth,(inT, outT)) -> 
+                                       "• [nth="^string_of_int (nth <: nat)^"]"
+                                       ^ "(" ^ S.concat ", " (T.map (fun t -> T.term_to_string (quote t)) inT) ^ "): " ^ T.term_to_string (quote outT)
+                                 ) l)
+                 )
+       else match l with
+       | [hd] -> fst hd
+       | _ -> let f (tt: _ {L.memP tt l}): T.Tac bool = subtype_tac (L.index inputs i) (L.index (fst (snd tt)) i) in
+             let l' = tfilter l f in
+             if Nil? l' then
+               ( let inputs_str: string = inputs_str () in
+                 let details = S.concat "\n" (T.map (fun (nth,(inT, outT)) ->
+                                              "• [nth="^string_of_int (nth <: nat)^"]"
+                                              ^ "(" ^ S.concat ", " (T.map (fun t -> T.term_to_string (quote t)) inT) ^ "): " ^ T.term_to_string (quote outT)
+                                        ) l) in
+                 T.fail ( error_header 4 ^ "Subtyping error: when calling a JavaScript function with "^string_of_int len^" arguments"
+                        ^ ", none of the following types matched the supplied arguments ("^inputs_str^"):\n"
+                        ));
+             while_multiple error_header inputs_str nb len inputs (i+1) l'
+
+let resolve_fun_signature
+  (sigs: list (list Type * Type)) (inputs: list Type)
+  : T.Tac (n:int{n < L.length sigs})
+  = let len = L.length inputs in
+    let sigs': l: list (nat * (list Type * Type)) {
+        forall x. L.memP x l ==> fst x < L.length sigs
+      } = withIndex sigs in
+    let correct_size: l: list (nat * (list Type * Type)) {
+        forall x. L.memP x l ==> (
+            L.length (fst (snd x)) == len
+          /\ fst x < L.length sigs'
+        )
+      }
+      = L.filter (fun (i, (inT, outT)) -> L.length inT = len) sigs' in
+    let inputs_str (): T.Tac string =
+      FStar.String.concat ", " (T.map (fun t -> "`" ^ T.term_to_string (quote t) ^ "`") inputs)
+    in
+    let error_header (code: nat) = "[resolve_fun_signature:E"^string_of_int code^"] " in
+    // let error (s: string): T.Tac unit = T.fail ( ^ s) in
+    if Nil? correct_size then
+      T.fail ( error_header 1 ^ "A JavaScript function was called with "
+             ^ string_of_int (L.length inputs) ^ " arguments ("
+             ^ inputs_str () ^ "), but the function in stake has " 
+             ^ string_of_int (L.length sigs)
+             ^ " overloadings, and none of them are of arity " ^ string_of_int (L.length inputs)
+             ^ "."
+             ^ "The overloadings of this JavaScript function are:\n"
+             ^ S.concat "\n" (T.map (fun (inT, outT) -> 
+                                   "• " ^ "(" ^ S.concat ", " (T.map (fun t -> T.term_to_string (quote t)) inT) ^ "): " ^ T.term_to_string (quote outT)
+                             ) sigs)
+             );
+    if len = 0 && L.length correct_size <> 1 then
+      T.fail ( error_header 2 ^ "A JavaScript function was called without argument"
+             ^ ", but it has multiple overloadings with zero arguments. "
+             ^ "The meta-program was not able to distinguish between them: you should "
+             ^ "set manually the meta-argument `nth` when calling the function."
+             ^ "The zero-arguments overloadings of this JavaScript function are:\n"
+             ^ S.concat "\n" (T.map (fun (nth,(inT, outT)) -> 
+                                   "• [nth="^string_of_int (nth <: nat)^"]"
+                                   ^ "(" ^ S.concat ", " (T.map (fun t -> T.term_to_string (quote t)) inT) ^ "): " ^ T.term_to_string (quote outT)
+                             ) correct_size)
+             );
+    while_multiple error_header inputs_str (L.length sigs') len inputs 0 correct_size
+
+(** Meta-programs that crafts a term w.r.t. `resolve_fun_signature`. *)
+let compute_fun_signature
+  (sigs: list (list Type * Type)) (inputs: list Type)
+  : T.Tac unit
+  = let n = resolve_fun_signature sigs inputs in
+    let n = quote n in
+    T.exact n
+
